Not 100% convinced

Std/Data/HashMap/Basic.lean
@@ -69,7 +69,10 @@ structure Imp (α : Type u) (β : Type v) where
   use the size to determine when to resize the map. -/
   size    : Nat
   /-- The bucket array of the `HashMap`. -/
-  buckets : Imp.Buckets α β
+  buckets : Array (AssocList α β)
+
+def Buckets.mk' : {m : Imp α β // 0 < m.2.size} → Imp.Buckets α β
+  | ⟨m, h⟩ => ⟨m.2, h⟩
 
 namespace Imp
 
@@ -81,16 +84,16 @@ A "load factor" of 0.75 is the usual standard for hash maps, so we return `capac
   capacity * 4 / 3
 
 /-- Constructs an empty hash map with the specified nonzero number of buckets. -/
-@[inline] def empty' (buckets := 8) (h : 0 < buckets := by decide) : Imp α β :=
-  ⟨0, .mk buckets h⟩
+@[inline] def empty' (buckets := 8) : Imp α β :=
+  ⟨0, mkArray buckets .nil⟩
 
 /-- Constructs an empty hash map with the specified target capacity. -/
-def empty (capacity := 0) : Imp α β :=
+def empty (capacity := 0) : {m : Imp α β // 0 < m.2.size} :=
   let nbuckets := numBucketsForCapacity capacity
   let n : {n : Nat // 0 < n} :=
     if h : nbuckets = 0 then ⟨8, by decide⟩
     else ⟨nbuckets, Nat.zero_lt_of_ne_zero h⟩
-  empty' n n.2
+  ⟨empty' n, by simpa [empty'] using n.2⟩
 
 /-- Calculates the bucket index from a hash value `u`. -/
 def mkIdx {n : Nat} (h : 0 < n) (u : USize) : {u : USize // u.toNat < n} :=
@@ -118,27 +121,29 @@ already in the array, which is appropriate when reinserting elements into the ar
   h.buckets.1.forM fun b => b.forM f
 
 /-- Given a key `a`, returns a key-value pair in the map whose key compares equal to `a`. -/
-def findEntry? [BEq α] [Hashable α] (m : Imp α β) (a : α) : Option (α × β) :=
+def findEntry? [BEq α] [Hashable α] (m : Imp α β) (h : 0 < m.2.size) (a : α) : Option (α × β) :=
   let ⟨_, buckets⟩ := m
-  let ⟨i, h⟩ := mkIdx buckets.2 (hash a |>.toUSize)
-  buckets.1[i].findEntry? a
+  let ⟨i, h⟩ := mkIdx h (hash a |>.toUSize)
+  buckets[i].findEntry? a
 
 /-- Looks up an element in the map with key `a`. -/
-def find? [BEq α] [Hashable α] (m : Imp α β) (a : α) : Option β :=
+def find? [BEq α] [Hashable α] (m : Imp α β) (h : 0 < m.2.size) (a : α) : Option β :=
   let ⟨_, buckets⟩ := m
-  let ⟨i, h⟩ := mkIdx buckets.2 (hash a |>.toUSize)
-  buckets.1[i].find? a
+  let ⟨i, h⟩ := mkIdx h (hash a |>.toUSize)
+  buckets[i].find? a
 
 /-- Returns true if the element `a` is in the map. -/
-def contains [BEq α] [Hashable α] (m : Imp α β) (a : α) : Bool :=
+def contains [BEq α] [Hashable α] (m : Imp α β) (h : 0 < m.2.size) (a : α) : Bool :=
   let ⟨_, buckets⟩ := m
-  let ⟨i, h⟩ := mkIdx buckets.2 (hash a |>.toUSize)
-  buckets.1[i].contains a
+  let ⟨i, h⟩ := mkIdx h (hash a |>.toUSize)
+  buckets[i].contains a
 
 /-- Copies all the entries from `buckets` into a new hash map with a larger capacity. -/
-def expand [Hashable α] (size : Nat) (buckets : Buckets α β) : Imp α β :=
+def expand [Hashable α] (size : Nat) (buckets : Buckets α β) :
+    {m : Imp α β // 0 < m.2.size} :=
   let nbuckets := buckets.1.size * 2
-  { size, buckets := go 0 buckets.1 (.mk nbuckets (Nat.mul_pos buckets.2 (by decide))) }
+  let ⟨arr, h⟩ := go 0 buckets.1 (.mk nbuckets (Nat.mul_pos buckets.2 (by decide)))
+  ⟨{ size, buckets := arr }, h⟩
 where
   /-- Inner loop of `expand`. Copies elements `source[i:]` into `target`,
   destroying `source` in the process. -/
@@ -158,53 +163,70 @@ where
 Inserts key-value pair `a, b` into the map.
 If an element equal to `a` is already in the map, it is replaced by `b`.
 -/
-@[inline] def insert [BEq α] [Hashable α] (m : Imp α β) (a : α) (b : β) : Imp α β :=
-  let ⟨size, buckets⟩ := m
-  let ⟨i, h⟩ := mkIdx buckets.2 (hash a |>.toUSize)
-  let bkt := buckets.1[i]
+@[inline] def insert [BEq α] [Hashable α] (m : Imp α β) (hm : 0 < m.2.size) (a : α) (b : β) :
+    {m : Imp α β // 0 < m.2.size} :=
+  let ⟨size, bucketArray⟩ := m
+  let buckets : Buckets α β := ⟨bucketArray, hm⟩
+  let ⟨i, h⟩ := mkIdx hm (hash a |>.toUSize)
+  let bkt := bucketArray[i]
   bif bkt.contains a then
-    ⟨size, buckets.update i (bkt.replace a b) h⟩
+    let ⟨newBucketArray, hnew⟩ := buckets.update i (bkt.replace a b) h
+    ⟨⟨size, newBucketArray⟩, hnew⟩
   else
     let size' := size + 1
-    let buckets' := buckets.update i (.cons a b bkt) h
+    let ⟨buckets', hnew⟩ := buckets.update i (.cons a b bkt) h
     if numBucketsForCapacity size' ≤ buckets.1.size then
-      { size := size', buckets := buckets' }
+      ⟨{ size := size', buckets := buckets' }, hnew⟩
     else
-      expand size' buckets'
+      expand size' ⟨buckets', hnew⟩
 
 /--
 Removes key `a` from the map. If it does not exist in the map, the map is returned unchanged.
 -/
-def erase [BEq α] [Hashable α] (m : Imp α β) (a : α) : Imp α β :=
-  let ⟨size, buckets⟩ := m
-  let ⟨i, h⟩ := mkIdx buckets.2 (hash a |>.toUSize)
-  let bkt := buckets.1[i]
-  bif bkt.contains a then ⟨size - 1, buckets.update i (bkt.erase a) h⟩ else ⟨size, buckets⟩
+def erase [BEq α] [Hashable α] (m : Imp α β) (hm : 0 < m.2.size) (a : α) :
+    {m : Imp α β // 0 < m.2.size} :=
+  let ⟨size, bucketArray⟩ := m
+  let buckets : Buckets α β := ⟨bucketArray, hm⟩
+  let ⟨i, h⟩ := mkIdx hm (hash a |>.toUSize)
+  let bkt := bucketArray[i]
+  bif bkt.contains a then
+    let ⟨newBuckets, hnew⟩ := buckets.update i (bkt.erase a) h
+    ⟨⟨size - 1, newBuckets⟩, hnew⟩
+  else
+    ⟨⟨size, bucketArray⟩, hm⟩
 
 /-- Map a function over the values in the map. -/
-@[inline] def mapVal (f : α → β → γ) (self : Imp α β) : Imp α γ :=
-  { size := self.size, buckets := self.buckets.mapVal f }
+@[inline] def mapVal (f : α → β → γ) (self : Imp α β) (hm : 0 < self.2.size) :
+    {m : Imp α γ // 0 < m.2.size} :=
+  let ⟨size, bucketArray⟩ := self
+  let buckets : Buckets α β := ⟨bucketArray, hm⟩
+  let ⟨newBucketArray, hnew⟩ := buckets.mapVal f
+  ⟨{ size := size, buckets := newBucketArray }, hnew⟩
 
 /-- Performs an in-place edit of the value, ensuring that the value is used linearly. -/
-def modify [BEq α] [Hashable α] (m : Imp α β) (a : α) (f : α → β → β) : Imp α β :=
-  let ⟨size, buckets⟩ := m
-  let ⟨i, h⟩ := mkIdx buckets.2 (hash a |>.toUSize)
-  let bkt := buckets.1[i]
+def modify [BEq α] [Hashable α] (m : Imp α β) (hm : 0 < m.2.size) (a : α) (f : α → β → β) :
+    {m : Imp α β // 0 < m.2.size} :=
+  let ⟨size, bucketArray⟩ := m
+  let buckets : Buckets α β := ⟨bucketArray, hm⟩
+  let ⟨i, h⟩ := mkIdx hm (hash a |>.toUSize)
+  let bkt := bucketArray[i]
   let buckets := buckets.update i .nil h -- for linearity
-  ⟨size, buckets.update i (bkt.modify a f) ((Buckets.update_size ..).symm ▸ h)⟩
+  let ⟨newBucketArray, hnew⟩ := buckets.update i (bkt.modify a f) ((Buckets.update_size ..).symm ▸ h)
+  ⟨⟨size, newBucketArray⟩, hnew⟩
 
 /--
 Applies `f` to each key-value pair `a, b` in the map. If it returns `some c` then
 `a, c` is pushed into the new map; else the key is removed from the map.
 -/
 @[specialize] def filterMap {α : Type u} {β : Type v} {γ : Type w}
-    (f : α → β → Option γ) (m : Imp α β) : Imp α γ :=
-  let m' := m.buckets.1.mapM (m := StateT (ULift Nat) Id) (go .nil) |>.run ⟨0⟩ |>.run
+    (m : Imp α β) (hm : 0 < m.2.size) (f : α → β → Option γ) :
+    {m : Imp α γ // 0 < m.2.size} :=
+  let m' := m.buckets.mapM (m := StateT (ULift Nat) Id) (go .nil) |>.run ⟨0⟩ |>.run
   have : m'.1.size > 0 := by
-    have := Array.size_mapM (m := StateT (ULift Nat) Id) (go .nil) m.buckets.1
+    have := Array.size_mapM (m := StateT (ULift Nat) Id) (go .nil) m.buckets
     simp [SatisfiesM_StateT_eq, SatisfiesM_Id_eq] at this
-    simp [this, Id.run, StateT.run, m.2.2, m']
-  ⟨m'.2.1, m'.1, this⟩
+    simp [this, Id.run, StateT.run, hm, m']
+  ⟨⟨m'.2.1, m'.1⟩, this⟩
 where
   /-- Inner loop of `filterMap`. Note that this reverses the bucket lists,
   but this is fine since bucket lists are unordered. -/
@@ -215,8 +237,9 @@ where
     | some c => go (.cons a c acc) l ⟨n.1 + 1⟩
 
 /-- Constructs a map with the set of all pairs `a, b` such that `f` returns true. -/
-@[inline] def filter (f : α → β → Bool) (m : Imp α β) : Imp α β :=
-  m.filterMap fun a b => bif f a b then some b else none
+@[inline] def filter (f : α → β → Bool) (m : Imp α β) (hm : 0 < m.2.size) :
+    {m : Imp α β // 0 < m.2.size} :=
+  m.filterMap hm fun a b => bif f a b then some b else none
 
 /--
 The well-formedness invariant for a hash map. The first constructor is the real invariant,
@@ -228,17 +251,32 @@ inductive WF [BEq α] [Hashable α] : Imp α β → Prop where
   * The `size` field should match the actual number of elements in the map
   * The bucket array should be well-formed, meaning that if the hashable instance
     is lawful then every element hashes to its index. -/
-  | mk : m.size = m.buckets.size → m.buckets.WF → WF m
+  | mk (m : Imp α β) :
+      (h : 0 < m.2.size) → m.size = Buckets.size ⟨m.2, h⟩ → Buckets.WF ⟨m.2, h⟩ → WF m
   /-- The empty hash map is well formed. -/
-  | empty' : WF (empty' n h)
+  | empty' : 0 < n → WF (empty' n)
   /-- Inserting into a well formed hash map yields a well formed hash map. -/
-  | insert : WF m → WF (insert m a b)
+  | insert : WF m → WF (insert m hm a b).1
   /-- Removing an element from a well formed hash map yields a well formed hash map. -/
-  | erase : WF m → WF (erase m a)
+  | erase : WF m → WF (erase m h a).1
   /-- Replacing an element in a well formed hash map yields a well formed hash map. -/
-  | modify : WF m → WF (modify m a f)
+  | modify : WF m → WF (modify m h a f).1
 
-theorem WF.empty [BEq α] [Hashable α] : WF (empty n : Imp α β) := by unfold empty; apply empty'
+theorem WF.empty [BEq α] [Hashable α] : WF ((Imp.empty n).1 : Imp α β) := by
+  dsimp only [Imp.empty]
+  split
+  · apply WF.empty'
+    simp
+  · next h =>
+    apply WF.empty'
+    exact Nat.pos_of_ne_zero h
+
+theorem WF.size [BEq α] [Hashable α] {m : Imp α β} : m.WF → 0 < m.2.size
+  | mk _ h _ _ => h
+  | empty' h => by simp [h, Imp.empty']
+  | insert _ => (Imp.insert _ _ _ _).2
+  | erase _ => (Imp.erase _ _ _).2
+  | modify _ => (Imp.modify _ _ _ _).2
 
 end Imp
 
@@ -255,7 +293,7 @@ open HashMap.Imp
 
 /-- Make a new hash map with the specified capacity. -/
 @[inline] def _root_.Std.mkHashMap [BEq α] [Hashable α] (capacity := 0) : HashMap α β :=
-  ⟨.empty capacity, .empty⟩
+  ⟨(Imp.empty capacity).1, .empty⟩
 
 instance [BEq α] [Hashable α] : Inhabited (HashMap α β) where
   default := mkHashMap
@@ -298,7 +336,8 @@ hashMap.insert "three" 3 = {"one" => 1, "two" => 2, "three" => 3}
 hashMap.insert "two" 0 = {"one" => 1, "two" => 0}
 ```
 -/
-def insert (self : HashMap α β) (a : α) (b : β) : HashMap α β := ⟨self.1.insert a b, self.2.insert⟩
+def insert (self : HashMap α β) (a : α) (b : β) : HashMap α β :=
+   ⟨self.1.insert self.2.size a b, self.2.insert⟩
 
 /--
 Similar to `insert`, but also returns a boolean flag indicating whether an existing entry has been
@@ -323,7 +362,8 @@ hashMap.erase "one" = {"two" => 2}
 hashMap.erase "three" = {"one" => 1, "two" => 2}
 ```
 -/
-@[inline] def erase (self : HashMap α β) (a : α) : HashMap α β := ⟨self.1.erase a, self.2.erase⟩
+@[inline] def erase (self : HashMap α β) (a : α) : HashMap α β :=
+  ⟨self.1.erase self.2.size a, self.2.erase⟩
 
 /--
 Performs an in-place edit of the value, ensuring that the value is used linearly.
@@ -334,7 +374,7 @@ The function `f` is passed the original key of the entry, along with the value i
 ```
 -/
 def modify (self : HashMap α β) (a : α) (f : α → β → β) : HashMap α β :=
-  ⟨self.1.modify a f, self.2.modify⟩
+  ⟨self.1.modify self.2.size a f, self.2.modify⟩
 
 /--
 Given a key `a`, returns a key-value pair in the map whose key compares equal to `a`.
@@ -346,7 +386,8 @@ hashMap.findEntry? "one" = some ("one", 1)
 hashMap.findEntry? "three" = none
 ```
 -/
-@[inline] def findEntry? (self : HashMap α β) (a : α) : Option (α × β) := self.1.findEntry? a
+@[inline] def findEntry? (self : HashMap α β) (a : α) : Option (α × β) :=
+  self.1.findEntry? self.2.size a
 
 /--
 Looks up an element in the map with key `a`.
@@ -356,7 +397,7 @@ hashMap.find? "one" = some 1
 hashMap.find? "three" = none
 ```
 -/
-@[inline] def find? (self : HashMap α β) (a : α) : Option β := self.1.find? a
+@[inline] def find? (self : HashMap α β) (a : α) : Option β := self.1.find? self.2.size a
 
 /--
 Looks up an element in the map with key `a`. Returns `b₀` if the element is not found.
@@ -390,7 +431,7 @@ hashMap.contains "one" = true
 hashMap.contains "three" = false
 ```
 -/
-@[inline] def contains (self : HashMap α β) (a : α) : Bool := self.1.contains a
+@[inline] def contains (self : HashMap α β) (a : α) : Bool := self.1.contains self.2.size a
 
 /--
 Folds a monadic function over the elements in the map (in arbitrary order).
@@ -483,7 +524,7 @@ def toArray (self : HashMap α β) : Array (α × β) :=
   self.fold (init := #[]) fun r k v => r.push (k, v)
 
 /-- The number of buckets in the hash map. -/
-def numBuckets (self : HashMap α β) : Nat := self.1.buckets.1.size
+def numBuckets (self : HashMap α β) : Nat := self.1.buckets.size
 
 /--
 Builds a `HashMap` from a list of key-value pairs.
